% Created 2016-09-15 Thu 16:21
\documentclass[11pt]{article}
\usepackage[utf8]{inputenc}
\usepackage[T1]{fontenc}
\usepackage{fixltx2e}
\usepackage{graphicx}
\usepackage{longtable}
\usepackage{float}
\usepackage{wrapfig}
\usepackage{rotating}
\usepackage[normalem]{ulem}
\usepackage{amsmath}
\usepackage{textcomp}
\usepackage{marvosym}
\usepackage{wasysym}
\usepackage{amssymb}
\usepackage{hyperref}
\tolerance=1000
\usepackage{listings}
\author{Daniel Dyla}
\date{\today}
\title{quiz1}
\hypersetup{
  pdfkeywords={},
  pdfsubject={},
  pdfcreator={Emacs 24.5.1 (Org mode 8.2.10)}}
\begin{document}

\maketitle
\tableofcontents

What does this function do and what is its runtime?

\lstset{language=Python,label= ,caption= ,numbers=none}
\begin{lstlisting}
def m(n):
    t = 1
    for i in range(n-1):
	for j in range(i+1, n):
	    t = 2*t
    return t
\end{lstlisting}

It returns $2^{r}$ where $r$ is the number of times $t = 2*t$ is
called (runtime).

\begin{align}
  T(n) &= \sum_{i=0}^{n-2} \sum_{j=i+1}^{n-1} 1 \\
  &= \sum_{i=0}^{n-2} (n-1) - (i+1) + 1 \\
  &= \sum_{i=0}^{n-2} (n - i - 1) \\
  &= \sum_{i=0}^{n-2} (n - 1) - \sum_{i=0}^{n-2} i \\
  &= (n - 1)(n - 2 - 0 + 1) - \frac{(n-2)(n-1)}{2} \\
  &= (n - 1)(n - 1) - \frac{(n-2)(n-1)}{2} \\
  &= (n-1)((n-1) - \frac{n-2}{2}) \\
  &= (n-2)(\frac{n}{n}) \\
  &= \frac{n(n-1)}{2}
\end{align}

Therefore, the function returns $2^{r}$ where $r = n(n-1)/2$.
% Emacs 24.5.1 (Org mode 8.2.10)
\end{document}
